wf for FOBV

lib/FirstOrderBitVec.v
@@ -78,6 +78,90 @@ Section FirstOrderBitVec.
     FirstOrder.mod_fns := mod_fns;
     FirstOrder.mod_rels := mod_rels;
   |}.
+
+  Definition output_wf (srt: sorts): mod_sorts srt -> Prop :=
+    match srt as srt' return mod_sorts srt' -> Prop with 
+    | Bits n => fun v => @n_tup_wf _ n v
+    end.
+
+
+  Fixpoint tm_wf {c srt} (t: tm c srt) : Prop :=
+    match t with
+    | TVar v => True
+    | @TFun _ c' args ret f hl =>
+      let rec := HList.all (fun srt => @tm_wf c' srt) hl in 
+      let fun_wf := 
+        match f with 
+        | BitsLit vs => n_tup_wf vs
+        | _ => True
+        end in 
+      rec /\ fun_wf
+    end.
+
+  Fixpoint valu_wf {c} (vs: valu _ fm_model c) : Prop :=
+    match vs with 
+    | VEmp _ _ => True
+    | VSnoc _ _ srt _ v inner  => 
+      output_wf srt v /\ valu_wf inner
+    end.
+
+  Fixpoint fm_wf {ctx} (e: fm ctx) : Prop := 
+    match e with 
+    | FTrue => True
+    | FFalse => True
+    | (FEq e1 e2) => tm_wf e1 /\ tm_wf e2
+    | (FRel _ _ _) => True
+    | (FNeg _ f) => fm_wf f
+    | (FOr _ f1 f2) => fm_wf f1 /\ fm_wf f2
+    | (FAnd _ f1 f2) => fm_wf f1 /\ fm_wf f2
+    | (FImpl f1 f2) => fm_wf f1 /\ fm_wf f2
+    | (FForall _ f) => fm_wf f
+    end.
+
+  Require Import Coq.Program.Tactics.
+  Require Import Coq.Program.Equality.
+
+  Lemma valu_find_wf : 
+    forall c srt (vs: valu _ _ c) v,
+      valu_wf vs -> 
+      output_wf srt (find _ fm_model v vs).
+  Proof.
+    intros.
+    dependent induction vs;
+    dependent destruction v;
+    autorewrite with find;
+    simpl in *;
+    intuition eauto.
+  Qed.
+
+  Lemma tm_interp_wf : 
+    forall c (v: valu _ _ c) srt (t: tm c srt), 
+      valu_wf v ->
+      tm_wf t -> 
+      output_wf srt (interp_tm (m := fm_model) v t).
+  Proof. 
+    dependent induction t using tm_ind'; intros;
+    autorewrite with interp_tm; try now (
+      eapply valu_find_wf; auto
+    ).
+
+    destruct srt eqn:?;
+    repeat match goal with 
+    | H: HList.t _ (_ :: _) |- _ => 
+      dependent destruction H
+    | H: HList.t _ nil |- _ => 
+      dependent destruction H
+    end; [ | | set (foo := (N.min (1 + hi) n - lo)%N) in *];
+    simpl;
+    [| | subst foo];
+    autorewrite with mod_fns;
+    simpl in *;
+    intuition eauto.
+    - eapply NtupleProofs.n_tup_cat_wf; 
+      intuition eauto.
+    - eapply NtupleProofs.n_tup_slice_wf;
+      intuition eauto.
+  Qed.
 End FirstOrderBitVec.
 
 
